LeanLoad/Plan/Init.lean
@@ -144,7 +144,7 @@ def plan (g : ObjectList) (layouts : Array ObjectLayout)
   for objectIdx in order do
     let some obj := g.val[objectIdx]?  | continue
     let some lyt := layouts[objectIdx]? | continue
-    let isExec := obj.elf.header.e_type = Elaborate.ET_EXEC
+    let isExec := obj.elf.elfType == .exec
     for entry in obj.elf.initArr do
       let fnAddr := if isExec then entry else lyt.base + entry
       if fnAddr != 0 then addrs := addrs.push fnAddr
